Date representation fixed and tested.

dateRep.dfy
@@ -4,28 +4,53 @@
 module DateRep 
 {
   // Start a 0 bc Dafny checks for 0, ask about witnesses
-  newtype Month = x : int | 0 <= x < 12
-  newtype Year = x : int | 0 <= x < 2019
-  newtype Day = x : int | 0 <= x < 31 
-  
-  method create(dd: int, mm: int, yyyy: int) returns(date: Date)
+  newtype Month = x : int | 0 < x <= 12 witness 1
+  newtype Year = x : int | 0 < x <= 2019 witness 1
+  newtype Day = x : int | 0 < x <= 31 witness 1
+
+  predicate validDate(dd: int, mm: int, yyyy: int)
   {
-    var d := Day(dd);
-    var m := Month(mm);
-    var y := Year(yyyy);
+    (0 <= mm < 12) && (0 <= yyyy < 2019) && (0 <= dd < 31)
+  }
+
+  method isValid(dd: int, mm: int, yyyy: int) returns (b:bool)
+  ensures b <==> validDate(dd, mm, yyyy)
+  {
+    b := ( (0 <= mm < 12) && (0 <= yyyy < 2019) && (0 <= dd < 31));
+  }
+
+  method create(dd: int, mm: int, yyyy: int) returns(date: Date)
+  requires validDate(dd, mm, yyyy)
+  requires 0 < dd <= 31
+  requires 0 < mm <= 12
+  requires 0 < yyyy <= 2019
+  {
+    assert validDate(dd, mm, yyyy);
+    var d := dd as Day;
+    var m := mm as Month;
+    var y := yyyy as Year;
     date := Date(d, m, y);
   }
     
   datatype Date = Date(day: Day, month: Month, year: Year)
 
   // Get current date
+  // idk how to implement 
   method current() returns (d: Date)
   {
-    return create(1, 10, 2019) // idk how to implement 
+    var day := 1;
+    var m := 10;
+    var y := 2018;
+    assert (0 <= day < 31);
+    assert (0 <= m < 12);
+    assert (0 <= y < 2019);
+    assert validDate(day,m,y);
+    
+    d := create(day,m,y); 
   }
 
   // d1 is before d2
-  method LessThan(d1:Date, d2:Date) returns (b: bool)
+  method lessThan(d1:Date, d2:Date) returns (b: bool)
   ensures b <==> (d1.year < d2.year) 
               || (d1.year == d2.year && d1.month < d2.month) 
               || (d1.year == d2.year && d1.month == d2.month && d1.day < d2.day) 
@@ -37,5 +62,22 @@ module DateRep
     // Compare years, overrides months if larger or uses previous to resolve tie
     b := (d2.year > d1.year) || (b && d2.year == d1.year);     
   }
+
+  // For testing module
+  /*
+  method Test()
+  {
+    var a := Date(1,12, 2014);
+    var b := Date(21, 1, 2015);
+
+    var test1 := lessThan(a, b);
+    var test2 := lessThan(b, a);
+    var test3 := lessThan(b, b);
+
+    assert (test1);
+    assert (!test2);    
+    assert (!test3);
+  }
+  */
 }
 
